very ugly (but complete) proofs
- I need to factor out the common lemmas related
  to mentionsU and instantiate and declare them
  somewhere.
- Maybe [mentionsU] should go into Expr?
- Maybe [instantiate] should go into Expr?

theories/STac/Apply.v
@@ -6,10 +6,10 @@ Require Import ExtLib.Tactics.
 Require Import MirrorCore.EnvI.
 Require Import MirrorCore.SymI.
 Require Import MirrorCore.SubstI3.
-Require Import MirrorCore.EProver2.
 Require Import MirrorCore.Lemma.
 Require Import MirrorCore.LemmaApply.
 Require Import MirrorCore.STac.Core.
+Require Import MirrorCore.STac.Continuation.
 
 Set Implicit Arguments.
 Set Strict Implicit.
@@ -21,43 +21,17 @@ Section parameterized.
   Variable RType_typ : RType typ.
   Variable Typ0_Prop : Typ0 _ Prop.
   Let tyProp : typ := @typ0 _ _ _ _.
+  Variable EqDec_eq_typ : EqDec typ (@eq typ).
 
   Variable vars_to_uvars : nat -> nat -> expr -> expr.
   Variable exprUnify : tenv typ -> tenv typ -> nat -> expr -> expr -> typ -> subst -> option subst.
   Variable instantiate : (nat -> option expr) -> nat -> expr -> expr.
+  Variable mentionsU : nat -> expr -> bool.
 
-  Section solve_but_last.
-    Variable Subst_subst : Subst subst expr.
-    Variables tus tvs : list typ.
-    Variable tac : stac typ expr subst.
-
-    Fixpoint solve_all_but_last
-             (hs : list expr) (es : list expr)
-             (sub : subst) {struct es}
-    : Result typ expr subst :=
-      match es with
-        | nil => @Solved _ _ _ nil nil sub
-        | e :: es =>
-          let e := instantiate (fun u => lookup u sub) 0 e in
-          match tac tus tvs sub hs e with
-            | Solved nil nil sub' =>
-              solve_all_but_last hs es sub'
-            | More tus tvs sub hs e =>
-              match es with
-                | nil => More tus tvs sub hs e
-                | _ => @Fail _ _ _
-              end
-            | _ => @Fail _ _ _
-          end
-      end.
-
-  End solve_but_last.
-
-  Section apply_other.
+  Section apply.
     Variable Subst_subst : Subst subst expr.
     Variable SU : SubstUpdate subst expr.
 
-    Definition fuel := 100.
     Let eapplicable :=
       @eapplicable typ expr tyProp subst vars_to_uvars
                    exprUnify.
@@ -68,9 +42,9 @@ Section parameterized.
      ** except the last are solved by the prover [tac], currently with
      ** empty facts.
      **)
-    Definition apply_other
+    Definition APPLY
                (lem : lemma typ expr expr)
-               (tac : stac typ expr subst)
+               (tacC : stac_cont typ expr subst)
     : stac typ expr subst :=
       let len_vars := length lem.(vars) in
       fun tus tvs sub hs e =>
@@ -78,18 +52,18 @@ Section parameterized.
         | None => @Fail _ _ _
         | Some sub' =>
           let len_uvars := length tus in
-          match pull (expr := expr) len_uvars len_vars sub' with
+          match pull (expr := expr) (SU := SU) len_uvars len_vars sub' with
             | Some sub'' =>
               let premises :=
                   map (fun e => instantiate (fun u => lookup u sub') 0
                                             (vars_to_uvars 0 len_uvars e))
                       lem.(premises)
               in
-              solve_all_but_last _ tus tvs tac hs premises sub''
+              tacC tus tvs sub'' hs premises
             | None => @Fail _ _ _
           end
       end.
-  End apply_other.
+  End apply.
 
   Variable Expr_expr : Expr RType_typ expr.
   Variable ExprOk_expr : ExprOk Expr_expr.
@@ -114,21 +88,35 @@ Section parameterized.
       val us (hlist_app vs vs') = val' (hlist_app us vs') vs).
 
   Hypothesis exprD'_instantiate
-  : forall f tus tvs e t P val,
-      (forall u t' get,
-         f u = Some e ->
-         nth_error_get_hlist_nth _ tus u = Some (existT _ t' get) ->
-         exists val,
-           exprD' tus tvs e t' = Some val ->
-           forall us vs,
-             P us vs ->
-             get us = val us vs) ->
-      exprD' tus tvs e t = Some val ->
-      exists val',
-        exprD' tus tvs (instantiate f 0 e) t = Some val' /\
-        forall us vs,
+  : forall tus tvs f e tvs' t eD P,
+      @sem_preserves_if _ _ _ Expr_expr tus tvs P f ->
+      exprD' tus (tvs' ++ tvs) e t = Some eD ->
+      exists eD',
+        exprD' tus (tvs' ++ tvs) (instantiate f (length tvs') e) t = Some eD' /\
+        forall us vs vs',
           P us vs ->
-          val us vs = val' us vs.
+          eD us (hlist_app vs' vs) = eD' us (hlist_app vs' vs).
+
+  Hypothesis exprD'_strengthen
+  : forall tus tu (e : expr) tvs (t : typ) eD,
+      mentionsU (length tus) e = false ->
+      exprD' (tus ++ tu :: nil) tvs e t = Some eD ->
+      exists eD',
+        exprD' tus tvs e t = Some eD' /\
+        forall us u vs,
+          eD (hlist_app us (Hcons u Hnil)) vs = eD' us vs.
+
+  Hypothesis instantiate_mentionsU
+  : forall f n e u,
+      mentionsU u (instantiate f n e) = true <->
+      (   (f u = None /\ mentionsU u e = true)
+       \/ exists u' e',
+            f u' = Some e' /\
+            mentionsU u' e = true/\
+            mentionsU u e' = true).
+
+  Hypothesis NormalizedSubst : NormalizedSubstOk mentionsU SubstOk_subst.
+
 
   Lemma exprD'_instantiate_substD
   : forall s tus tvs e t P val,
@@ -141,194 +129,31 @@ Section parameterized.
           P us vs ->
           val us vs = val' us vs.
   Proof.
-    intros. eapply exprD'_instantiate in H1; eauto.
-    { simpl. clear - H H0. intros.
-      eapply substD_lookup in H0; eauto.
+    intros.
+    eapply exprD'_instantiate
+      with (tvs' := nil) (f := fun u => lookup u s) (P:=P)
+      in H1.
+    { clear - H H0 H1. simpl in *.
+      forward_reason. eexists; split; eauto.
+      intros. specialize (H2 us vs Hnil).
+      apply H2; auto. }
+    { red. intros.
+      eapply substD_lookup in H2; eauto.
+      eapply nth_error_get_hlist_nth_Some in H3.
+      simpl in *.
       forward_reason.
-      eapply nth_error_get_hlist_nth_Some in H2.
-      simpl in H2.
-      destruct H2.
-      assert (x = t').
+      assert (x = t0).
       { clear - x2 x1. rewrite <- x1 in x2.
         inv_all; auto. }
       subst.
-      eexists; split; eauto. }
+      eexists; split; eauto.
+      intros. eapply H4 in H5; clear H4.
+      rewrite H3.
+      rewrite H5.
+      clear - EqDec_eq_typ.
+      destruct x1.
+      rewrite (UIP_refl x2). reflexivity. }
   Qed.
-
-  (** TODO: This is not correct anymore **)
-(*
-  Theorem solve_all_but_last_sound
-  : forall tus tvs (tac : stac typ expr subst) (hs prems : list expr) (sub : subst),
-      stac_sound tac ->
-      WellFormed_subst sub ->
-      match solve_all_but_last _ tus tvs tac hs prems sub with
-        | Fail => True
-        | Solved tus' tvs' s' =>
-          WellFormed_subst s' /\
-          match mapT (F := option) (T := list) (goalD Expr_expr Typ0_Prop tus tvs) prems with
-            | Some Gs =>
-              match substD tus tvs sub with
-                | Some sV =>
-                  match substD (tus ++ tus') (tvs ++ tvs') s' with
-                    | Some s'V =>
-                      forall (us : hlist (typD nil) tus)
-                             (vs : hlist (typD nil) tvs),
-                        (exists
-                            (us' : hlist (typD nil) tus')
-                            (vs' : hlist (typD nil) tvs'),
-                            s'V (hlist_app us us') (hlist_app vs vs')) ->
-                        Forall (fun G => G us vs) Gs /\ sV us vs
-                    | None => False
-                  end
-                | None => True
-              end
-            | None => True
-          end
-        | More tus' tvs' s' hs' g' =>
-          WellFormed_subst s' /\
-          match mapT (F := option) (T := list) (goalD Expr_expr Typ0_Prop tus tvs) prems with
-            | Some Gs =>
-              match substD tus tvs sub with
-                | Some sV =>
-                  match goalD Expr_expr Typ0_Prop (tus ++ tus') (tvs ++ tvs') g' with
-                    | Some G' =>
-                      match substD (tus ++ tus') (tvs ++ tvs') s' with
-                        | Some s'V =>
-                          forall (us : hlist (typD nil) tus)
-                                 (vs : hlist (typD nil) tvs),
-                            (exists
-                                (us' : hlist (typD nil) tus')
-                                (vs' : hlist (typD nil) tvs'),
-                                s'V (hlist_app us us') (hlist_app vs vs') /\
-                                G' (hlist_app us us') (hlist_app vs vs')) ->
-                            Forall (fun G => G us vs) Gs /\ sV us vs
-                        | None => False
-                      end
-                    | None => False
-                  end
-                | None => True
-              end
-            | None => True
-          end
-      end.
-  Proof.
-    Opaque mapT.
-    intros. generalize dependent sub.
-    induction prems.
-    { simpl. forward.
-      rewrite list_mapT_nil in H0.
-      split; auto.
-      inv_all; subst.
-      repeat match goal with
-               | |- match ?X with _ => _ end =>
-                 consider X; intros; auto
-             end.
-      { split. constructor.
-        destruct H3 as [ ? [ ? ? ] ].
-        rewrite (hlist_eta x) in *.
-        rewrite (hlist_eta x0) in *.
-        do 2 rewrite hlist_app_nil_r in H3.
-        destruct (eq_sym (app_nil_r_trans tus)).
-        destruct (eq_sym (app_nil_r_trans tvs)).
-        rewrite H0 in H2. inv_all. subst. assumption. }
-      { destruct (eq_sym (app_nil_r_trans tus)).
-        destruct (eq_sym (app_nil_r_trans tvs)). congruence. } }
-    { intros.
-      simpl.
-      specialize (H tus tvs sub (instantiate (fun u : nat => lookup u sub) 0 a)).
-      destruct (tac tus tvs sub (instantiate (fun u : nat => lookup u sub) 0 a)); auto.
-      { forward; subst.
-        forward_reason.
-        specialize (IHprems _ H).
-        destruct (solve_all_but_last Subst_subst tus tvs tac prems s); auto.
-        { forward_reason.
-          split; auto.
-          rewrite list_mapT_cons.
-          unfold goalD in *.
-          forward. inv_all; subst.
-          eapply exprD'_instantiate_substD with (s := sub) in H4; eauto.
-          { forward_reason.
-            rewrite H4 in *.
-            forward.
-            consider (substD tus tvs s); intros.
-            { forward.
-              specialize (H9 us vs).
-              destruct H9.
-              { do 2 exists Hnil. revert H7.
-                eapply H10 in H11.
-                revert H5. destruct H11.
-                revert H7.
-                clear.
-                do 2 rewrite hlist_app_nil_r.
-                destruct (eq_sym (app_nil_r_trans tus)).
-                destruct (eq_sym (app_nil_r_trans tvs)).
-                intros. rewrite H5 in *. inv_all; subst; auto. }
-              { split; auto.
-                constructor.
-                { repeat rewrite eq_Arr_eq in *. repeat rewrite eq_Const_eq in *.
-                  rewrite H6; eauto. }
-                { eapply H10 in H11. forward_reason. assumption. } } }
-            { clear - H5 H7.
-              exfalso.
-              destruct (eq_sym (app_nil_r_trans tus)).
-              destruct (eq_sym (app_nil_r_trans tvs)). congruence. } } }
-        { rewrite list_mapT_cons.
-          forward_reason.
-          split; eauto.
-          unfold goalD in *.
-          forward.
-          inv_all; subst.
-          eapply exprD'_instantiate_substD with (s := sub) in H4; eauto.
-          forward_reason.
-          rewrite H4 in *.
-          forward.
-          consider (substD tus tvs s).
-          { intros; forward.
-            inv_all; subst.
-            eapply H11 in H12; clear H11.
-            specialize (H9 us vs).
-            destruct H12.
-            destruct H9.
-            { do 2 exists Hnil.
-              do 2 rewrite hlist_app_nil_r.
-              destruct (eq_sym (app_nil_r_trans tus)).
-              destruct (eq_sym (app_nil_r_trans tvs)).
-              rewrite H7 in *. inv_all; subst. assumption. }
-            { split; auto.
-              constructor; auto.
-              revert H9.
-              repeat rewrite eq_Arr_eq.
-              repeat rewrite eq_Const_eq.
-              rewrite H6; auto. } }
-          { intro; exfalso.
-            revert H7 H5. clear.
-            destruct (eq_sym (app_nil_r_trans tus)).
-            destruct (eq_sym (app_nil_r_trans tvs)). congruence. } } }
-      { destruct prems; auto.
-        destruct H; auto.
-        split; auto.
-        rewrite list_mapT_cons. rewrite list_mapT_nil.
-        clear IHprems.
-        unfold goalD in *.
-        forward.
-        inv_all; subst.
-        eapply exprD'_instantiate_substD with (s := sub) in H2; eauto.
-        { forward_reason.
-          rewrite H2 in *.
-          forward. inv_all; subst.
-          forward_reason.
-          specialize (H6 us vs). destruct H6.
-          { exists x0; exists x1.
-            split; auto. }
-          { split; auto.
-            constructor; auto.
-            revert H6.
-            repeat rewrite eq_Arr_eq.
-            repeat rewrite eq_Const_eq.
-            rewrite H3; auto. } } } }
-    Transparent mapT.
-  Qed.
-*)
 
   Lemma mapT_map : forall T U V (f : U -> option V) (g : T -> U) ls,
                      mapT f (map g ls) = mapT (fun x => f (g x)) ls.
@@ -338,6 +163,7 @@ Section parameterized.
     destruct (f (g a)); auto.
     rewrite IHls. reflexivity.
   Qed.
+
   Lemma map_mapT : forall T U V (f : T -> option U) (g : U -> V) ls,
                      match mapT f ls with
                        | None => None
@@ -353,6 +179,7 @@ Section parameterized.
     rewrite <- IHls.
     destruct (mapT f ls); auto.
   Qed.
+
   Lemma mapT_ext : forall T U (f g : T -> option U),
                      (forall x, f x = g x) ->
                      forall (ls : list T),
@@ -363,8 +190,9 @@ Section parameterized.
     rewrite H. rewrite IHls. destruct (g a); auto.
   Qed.
 
-  Lemma join_env_app : forall ts a b (ax : hlist _ a) (bx : hlist _ b),
-                         join_env ax ++ join_env (ts := ts) bx = join_env (hlist_app ax bx).
+  Lemma join_env_app
+  : forall ts a b (ax : hlist _ a) (bx : hlist _ b),
+      join_env ax ++ join_env (ts := ts) bx = join_env (hlist_app ax bx).
   Proof.
     clear.
     induction ax; simpl; intros; auto.
@@ -386,101 +214,115 @@ Section parameterized.
       | eq_refl => P
     end.
 
+  Lemma lemmaD'_convert
+  : forall tyProp concl lem F G H tus tvs P,
+      (forall x y z, F x y z = G x y z) ->
+      lemmaD' (tyProp := tyProp) (conclusion := concl) Expr_expr F H tus tvs lem = Some P ->
+      lemmaD' Expr_expr G H tus tvs lem = Some P.
+  Proof.
+    clear.
+    destruct lem. intros. revert H1. Opaque mapT.
+    unfold lemmaD'. simpl.
+    unfold goalD. unfold ResType.
+    repeat rewrite eq_option_eq.
+    match goal with
+      | |- match ?X with _ => _ end = _ -> match ?Y with _ => _ end = _ =>
+        change Y with X ; generalize X
+    end.
+    destruct o; try congruence.
+    rewrite H0.
+    destruct (G tus (vars ++ tvs) concl0); try congruence.
+  Qed.
+
+  Lemma goalD_weakenU
+  : forall (tus0 tvs0 : tenv typ) (l0 : expr)
+           (lD : hlist (typD nil) tus0 -> hlist (typD nil) tvs0 -> Prop),
+      goalD tus0 tvs0 l0 = Some lD ->
+      forall tus' : list typ,
+      exists
+        lD' : hlist (typD nil) (tus0 ++ tus') -> hlist (typD nil) tvs0 -> Prop,
+        goalD (tus0 ++ tus') tvs0 l0 = Some lD' /\
+        (forall (us : hlist (typD nil) tus0) (us' : hlist (typD nil) tus')
+                (vs : hlist (typD nil) tvs0), lD us vs <-> lD' (hlist_app us us') vs).
+  Proof.
+    unfold goalD. clear - ExprOk_expr.
+    intros. forward. inv_all; subst.
+    eapply exprD'_weakenU with (tus' := tus') in H; eauto.
+    forward_reason. rewrite H.
+    eexists; split; eauto. intros.
+    repeat first [ rewrite eq_Const_eq in *
+                 | rewrite eq_option_eq in *
+                 | rewrite eq_Arr_eq in * ].
+    rewrite <- H0.
+    reflexivity.
+  Qed.
+
   Theorem APPLY_sound
-  : forall lem tac,
+  : forall lem tacC,
       @lemmaD typ _ expr _ expr (@goalD _ _ _ _ _ ) (@typ0 _ _ _ _)
               (fun P => match typ0_cast nil in _ = T return T
                         with
                           | eq_refl => P
                         end)
               nil nil lem ->
-      stac_sound tac ->
-      stac_sound (apply_other _ _ lem tac).
+      stac_cont_sound tacC ->
+      stac_sound (APPLY _ _ lem tacC).
   Proof.
     intros. red. intros.
-    unfold apply_other.
+    unfold APPLY.
     consider (eapplicable tyProp vars_to_uvars exprUnify s tus tvs lem g); auto; intros.
     eapply (@eapplicable_sound _ _ _ _ _ tyProp (@typ0_cast _ _ _ _)) in H2; eauto.
-    destruct H2.
-    red in H. simpl in H. forward.
-    eapply pull_sound in H5; eauto.
-    destruct H5.
-(*
-    generalize (@solve_all_but_last_sound tus tvs tac
-                                          (map (fun e : expr =>
-                                                  instantiate (fun u : nat => lookup u s0) 0
-                                                              (vars_to_uvars 0 (length tus) e)) (premises lem))
-                                          s1 H0 H5).
-    consider (substD tus tvs s).
-    { consider (goalD Expr_expr Typ0_Prop tus tvs g).
-      { intros.
-        assert (lemmaD' Expr_expr
-                        (fun (tus0 tvs0 : tenv typ) (g0 : expr) =>
-                           match typ0_cast nil in (_ = t) return (ResType tus0 tvs0 t) with
-                             | eq_refl => exprD' tus0 tvs0 g0 tyProp
-                           end)
-                        (fun x : typD nil tyProp =>
-                           match typ0_cast nil in (_ = t) return t with
-                             | eq_refl => x
-                           end) nil nil lem = Some P).
-        { clear - H.
-          unfold lemmaD', goalD in *.
-          match goal with
-            | H : match ?X with _ => _ end = _ |- match ?Y with _ => _ end = _ =>
-              change Y with X; consider X; try congruence; intros
-          end.
-          unfold ResType.
-          rewrite eq_option_eq.
-          eauto. }
-        clear H.
-        unfold goalD in *. forward.
-        specialize (H8 _ _ _ H10 eq_refl H).
+    forward_reason.
+    red in H. simpl in H.
+    consider (pull (length tus) (length (vars lem)) s0); auto; [ ].
+    intros.
+    match goal with
+      | |- match tacC ?A ?B ?C ?D ?E with _ => _ end =>
+        specialize (H0 A B C D E)
+    end.
+    eapply pull_for_instantiate_sound
+      with (instantiate := instantiate) (mentionsU := mentionsU)
+           (tvs := tvs) in H4; eauto.
+    forward_reason.
+    { do 3 match goal with
+             | |- context [ match ?X with Some _ => _ | None => True end ] =>
+               consider X ; [ intros | solve [ intuition forward ] ]
+           end.
+      unfold goalD in H6.
+      forward.
+      eapply H8 in H6; clear H8; eauto.
+      { forward_reason.
+        eapply lemmaD'_weakenU with (tus' := tus) in H; eauto using goalD_weakenU.
+        specialize (H5 _ H6).
         forward_reason.
-        specialize (H6 _ _ _ _ eq_refl eq_refl H8).
-        forward_reason. inv_all. subst.
-        eapply lemmaD'_weakenU with (tus' := tus) in H10; eauto.
-        { forward_reason.
-          unfold lemmaD' in H3. Opaque mapT. simpl in H3.
-          unfold ResType in H3. rewrite eq_option_eq in H3.
-          forward. inv_all; subst.
-          assert (exists ZZ,
-                    mapT (T:=list) (F:=option)
-                         (fun goal : expr =>
-                            match exprD' (Expr := Expr_expr) tus tvs goal (typ0 (F:=Prop)) with
-                              | Some val =>
-                                Some
-                                  match
-                                    typ0_cast nil in (_ = T)
-                                    return
-                                    (hlist (typD nil) tus -> hlist (typD nil) tvs -> T)
-                                  with
-                                    | eq_refl => val
-                                  end
-                              | None => None
-                            end)
-                         (map
-                            (fun e : expr =>
-                               instantiate (fun u : nat => lookup u s0) 0
-                                           (vars_to_uvars 0 (length tus) e)) 
-                            (premises lem)) = Some ZZ /\
-                    forall us vs ls,
-                      x (hlist_app us ls) vs ->
-                      Forall2 (fun x y =>
-                                 match typ0_cast nil in _ = T return T with
-                                   | eq_refl => x us (hlist_app ls Hnil)
-                                 end <-> y us vs) l ZZ).
-        { clear H17 H10.
+        rewrite H5 in *.
+        unfold lemmaD' in H. forward.
+        assert (exists ZZ,
+                  mapT (T:=list) (F:=option) (goalD tus tvs)
+                       (map
+                          (fun e : expr =>
+                             instantiate (fun u : nat => lookup u s0) 0
+                                         (vars_to_uvars 0 (length tus) e))
+                          (premises lem)) = Some ZZ /\
+                  forall us vs ls,
+                    x (hlist_app us ls) vs ->
+                    Forall2 (fun x y =>
+                               match typ0_cast nil in _ = T return T with
+                                 | eq_refl => x us (hlist_app ls Hnil)
+                               end <-> y us vs) l0 ZZ).
+        { clear H14 H15 H7.
           rewrite mapT_map.
+          unfold goalD.
           rewrite <- map_mapT.
-          revert H3. revert l.
+          revert H. revert l0.
           induction (premises lem).
           { do 2 rewrite list_mapT_nil. simpl.
             intros. inv_all. subst. eexists; split; eauto. }
           { do 2 rewrite list_mapT_cons. intros.
             forward; inv_all; subst.
-            specialize (IHl _ eq_refl). forward_reason.
+            specialize (IHl0 _ eq_refl). forward_reason.
             forward.
-            eapply vars_to_uvars_sound with (tvs0 := nil) in H3.
+            eapply vars_to_uvars_sound with (tvs0 := nil) in H.
             forward_reason.
             assert (substD (tus ++ vars lem ++ nil) tvs s0 =
                     Some match eq_sym (app_nil_r_trans (vars lem)) in _ = T
@@ -488,83 +330,189 @@ Section parameterized.
                          with
                            | eq_refl => x
                          end).
-            { revert H8. clear.
+            { revert H6. clear.
               destruct (eq_sym (app_nil_r_trans (vars lem))). auto. }
-            eapply exprD'_weakenV with (tvs' := tvs) in H3; eauto.
-            destruct H3 as [ ? [ ? ? ] ]. simpl in H3.
-            eapply exprD'_instantiate_substD with (s := s0) in H3; eauto.
-            destruct H3 as [ ? [ ? ? ] ].
-            admit. } }
-        { destruct H12 as [ ? [ ? ? ] ].
-          match goal with
-            | H : context [ ?X ] , H' : ?Y = _ |- _ =>
-              change X with Y in H ; rewrite H' in H
-          end.
-          match goal with
-            | H : match ?X with _ => _ end |- match ?Y with _ => _ end =>
-              change Y with X ; consider X; auto
-          end; intros; forward.
-          { forward_reason; split; auto.
-            intros. eapply H19 in H20; clear H19.
+            eapply exprD'_weakenV with (tvs' := tvs) in H; eauto.
+            forward_reason. simpl in H.
+            pose (pfu := match app_nil_r_trans (vars lem) in _ = T
+                               return tus ++ T = tus ++ vars lem ++ nil
+                         with
+                           | eq_refl => eq_refl
+                         end).
+            rewrite exprD'_conv with (pfv := eq_refl) (pfu := pfu) in H.
+            subst pfu.
+            unfold ResType in H. rewrite eq_option_eq in H.
+            forward.
+            eapply H12 in H.
             forward_reason.
-            eapply H13 in H20; clear H13. (*
-            specialize (H15 _ _ _ H20).
-            specialize (H11 _ _ _ H20); clear H20.
-            forward_reason. split; auto.
-            unfold exprD in H11.
-            rewrite join_env_app in H11.
-            repeat rewrite split_env_join_env in H11.
+            rewrite H.
+            eexists; split; eauto.
+            intros.
+            simpl. constructor.
+            { repeat first [ rewrite eq_Const_eq | rewrite eq_Arr_eq ].
+              rewrite <- (H21 us vs ls); clear H21; auto.
+              generalize (H16 us (hlist_app ls Hnil) Hnil); clear H16.
+              generalize (H18 (hlist_app us (hlist_app ls Hnil)) Hnil vs); clear H18.
+              inv_all. subst.
+              clear. simpl.
+              intros. rewrite H0; clear H0.
+              change_rewrite H; clear H.
+              match goal with
+                | |- ?X <-> ?Y =>
+                  cutrewrite (X = Y); [ reflexivity | ]
+              end.
+              eapply match_eq_match_eq with (F := fun x => x).
+              repeat first [ rewrite eq_Const_eq | rewrite eq_Arr_eq ].
+              f_equal.
+              rewrite hlist_app_nil_r.
+              clear. revert ls.
+              generalize (app_nil_r_trans (vars lem)).
+              destruct e. reflexivity. }
+            { inv_all. subst. eauto. } } }
+        { forward_reason.
+          change_rewrite H16 in H7.
+          unfold exprD in H8.
+          consider (tacC tus tvs s1 hs
+                         (map
+                            (fun e : expr =>
+                               instantiate (fun u : nat => lookup u s0) 0
+                                           (vars_to_uvars 0 (length tus) e)) (premises lem))); auto.
+          { intros. forward_reason; split; auto.
+            forward.
+            eapply H20 in H22; eauto. clear H20 H21.
+            inv_all; subst.
+            specialize (H13 us vs).
+            forward_reason. rewrite H9 in H15; clear H9.
+            generalize (H17 _ _ _ H15); clear H17.
+            generalize(H8 _ _ _ H15); clear H8.
+            rewrite join_env_app.
+            do 2 rewrite split_env_join_env.
+            intros; forward_reason; split; auto.
             forward. inv_all; subst.
             repeat first [ rewrite eq_Const_eq | rewrite eq_Arr_eq ].
             rewrite <- H20; clear H20.
-            specialize (H10 Hnil us Hnil).
-            eapply H10 in H4; clear H10. simpl in H4.
-            rewrite foralls_sem in H4.
-            specialize (H4 (hlist_map
-               (fun (t2 : typ)
-                  (x4 : hlist (typD nil) tus ->
-                        hlist (typD nil) tvs -> typD nil t2) => 
-                x4 us vs) x2)).
-            repeat first [ rewrite eq_Const_eq in H4 | rewrite eq_Arr_eq in H4 ].
-            eapply exprD'_weakenV with (tvs' := tvs) in H14; eauto.
-            destruct H14 as [ ? [ ? ? ] ].
-            assert (x4 = match eq_sym (app_nil_r (vars lem)) in _ = T
-                               return hlist _ tus -> hlist _ (T ++ tvs) -> _
-                         with
-                           | eq_refl => t1
-                         end).
-            { generalize dependent (concl lem).
-              clear. destruct (eq_sym (app_nil_r (vars lem))).
-              congruence. }
-            subst.
-            specialize (H14 us (hlist_app (hlist_map
-               (fun (t2 : typ)
-                  (x4 : hlist (typD nil) tus ->
-                        hlist (typD nil) tvs -> typD nil t2) => 
-                x4 us vs) x2) Hnil) vs). *)
-            admit. }
-          { admit. } } }
-        { clear - ExprOk_expr. unfold ResType. intros.
-          repeat rewrite eq_option_eq in *.
-          forward. eapply exprD'_weakenU with (tus' := tus') in H; eauto.
-          destruct H as [ ? [ ? ? ] ].
-          rewrite H. eexists; split; eauto.
-          intros. inv_all; subst.
-          repeat first [ rewrite eq_Const_eq | rewrite eq_Arr_eq ].
-          rewrite <- H1. reflexivity. } }
-      { intros. revert H9.
-        match goal with
-          | |- match ?X with _ => _ end -> match ?Y with _ => _ end =>
-            change Y with X; consider X; intros
-        end; auto;
-        forward_reason; split; auto; forward. } }
-    { intros. revert H8.
-      match goal with
-        | |- match ?X with _ => _ end -> match ?Y with _ => _ end =>
-          change Y with X; consider X; intros
-      end; auto;
-      forward_reason; split; auto; forward. }
-*)
-  Admitted.
+            eapply H11 with (us' := us) in H10; clear H11.
+            rewrite foralls_sem in H10.
+            specialize (H10 x0).
+            rewrite impls_sem in H10.
+            rewrite Forall_map in H10.
+            cut (P2 us (hlist_app x0 Hnil)).
+            { revert H8 H14. simpl. clear - ExprOk_expr.
+              unfold goalD. intros; forward.
+              inv_all; subst.
+              eapply exprD'_weakenV with (tvs' := tvs) in H0; eauto.
+              forward_reason.
+              rewrite exprD'_conv
+                 with (pfu := eq_refl)
+                      (pfv := match app_nil_r_trans (vars lem) in _ = T return T ++ tvs = (vars lem ++ nil) ++ tvs
+                              with
+                                | eq_refl => eq_refl
+                              end) in H0.
+              unfold ResType in H0.
+              specialize (H1 us (hlist_app x0 Hnil) vs).
+              repeat first [ rewrite eq_Const_eq in *
+                           | rewrite eq_option_eq in *
+                           | rewrite eq_Arr_eq in * ].
+              change_rewrite H8 in H0.
+              inv_all; subst.
+              repeat first [ rewrite eq_Const_eq in *
+                           | rewrite eq_option_eq in *
+                           | rewrite eq_Arr_eq in * ].
+              rewrite H1 in H; clear H1.
+              revert H; clear.
+              rewrite hlist_app_nil_r.
+              match goal with
+                | |- ?X -> ?Y =>
+                  cutrewrite (X = Y); auto
+              end.
+              eapply match_eq_match_eq with (F := fun x => x).
+              f_equal.
+              clear.
+              generalize (app_nil_r_trans (vars lem)).
+              generalize dependent (vars lem).
+              intro. generalize dependent (l ++ nil).
+              intros; subst. reflexivity. }
+            { eapply H10.
+              revert H9 H13. clear.
+              induction 1.
+              { constructor. }
+              { inversion 1; subst.
+                constructor; auto.
+                eapply H. assumption. } } }
+          { (** TODO(gmalecha): Abstract this proof **)
+            intros. forward_reason; split; auto.
+            forward.
+            inv_all; subst.
+            specialize (H13 us vs).
+            eapply H22 in H24; eauto; clear H22 H23; [ ].
+            specialize (H11 Hnil us Hnil).
+            eapply H11 in H10; clear H11.
+            forward_reason. rewrite H9 in H13; clear H9.
+            generalize (H17 _ _ _ H13); clear H17.
+            generalize(H8 _ _ _ H13); clear H8.
+            rewrite join_env_app.
+            do 2 rewrite split_env_join_env.
+            intros; forward_reason; split; auto.
+            forward. inv_all; subst.
+            repeat first [ rewrite eq_Const_eq | rewrite eq_Arr_eq ].
+            rewrite <- H17; clear H17.
+            rewrite foralls_sem in H10.
+            specialize (H10 x0).
+            rewrite impls_sem in H10.
+            rewrite Forall_map in H10.
+            cut (P2 us (hlist_app x0 Hnil)).
+            { (** TODO(gmalech): This is definitely abstractable **)
+              revert H8 H14. simpl. clear - ExprOk_expr.
+              unfold goalD. intros; forward.
+              inv_all; subst.
+              eapply exprD'_weakenV with (tvs' := tvs) in H0; eauto.
+              forward_reason.
+              rewrite exprD'_conv
+                 with (pfu := eq_refl)
+                      (pfv := match app_nil_r_trans (vars lem) in _ = T return T ++ tvs = (vars lem ++ nil) ++ tvs
+                              with
+                                | eq_refl => eq_refl
+                              end) in H0.
+              unfold ResType in H0.
+              specialize (H1 us (hlist_app x0 Hnil) vs).
+              repeat first [ rewrite eq_Const_eq in *
+                           | rewrite eq_option_eq in *
+                           | rewrite eq_Arr_eq in * ].
+              change_rewrite H8 in H0.
+              inv_all; subst.
+              repeat first [ rewrite eq_Const_eq in *
+                           | rewrite eq_option_eq in *
+                           | rewrite eq_Arr_eq in * ].
+              rewrite H1 in H; clear H1.
+              revert H; clear.
+              rewrite hlist_app_nil_r.
+              match goal with
+                | |- ?X -> ?Y =>
+                  cutrewrite (X = Y); auto
+              end.
+              eapply match_eq_match_eq with (F := fun x => x).
+              f_equal.
+              clear.
+              generalize (app_nil_r_trans (vars lem)).
+              generalize dependent (vars lem).
+              intro. generalize dependent (l ++ nil).
+              intros; subst. reflexivity. }
+            { eapply H10.
+              revert H9 H11. clear.
+              induction 1.
+              { constructor. }
+              { inversion 1; subst.
+                constructor; auto.
+                eapply H. assumption. } } } } }
+      { clear - H.
+        eapply lemmaD'_convert; [ | eassumption ].
+        unfold goalD. simpl.
+        intros; forward.
+        inv_all; subst.
+        unfold tyProp.
+        destruct (exprD' x y z (typ0 (F:=Prop))).
+        unfold ResType. rewrite eq_option_eq. reflexivity.
+        unfold ResType. rewrite eq_option_eq. reflexivity. } }
+  Qed.
 
 End parameterized.
