theories/STac/STac.v
@@ -9,3 +9,4 @@ Require Export MirrorCore.STac.Fail.
 Require Export MirrorCore.STac.Rec.
 Require Export MirrorCore.STac.Apply.
 Require Export MirrorCore.STac.Simplify.
+Require Export MirrorCore.STac.UseForAll.
